lib/Lib.Buffer.fsti
@@ -756,10 +756,10 @@ val loop_blocks:
       Seq.repeat_blocks #a #(Seq.lseq b (v blen)) (v blocksize) (as_seq h0 inp) spec_f spec_l (as_seq h0 write))
 
 open FStar.Mul
-
+(*
 (** Fills a buffer block by block using a function with an accumulator *)
 inline_for_extraction noextract
-val fill_blocks:
+val fill_blocks_:
     #t:Type0
   -> h0:mem
   -> len:size_t
@@ -788,6 +788,40 @@ val fill_blocks:
       B.modifies (B.loc_union (footprint (v n)) (loc output)) h0 h1 /\
       refl h1 (v n) == s /\
       as_seq #_ #t h1 (gsub output (size 0) (n *! len)) == o)
+*)
+
+(** Fills a buffer block by block using a function with an accumulator *)
+inline_for_extraction noextract
+val fill_blocks:
+    #t:Type0
+  -> h0:mem
+  -> len:size_t
+  -> n:size_t{v n * v len <= max_size_t}
+  -> output:lbuffer t (n *! len)
+  -> a_spec:(i:size_nat{i <= v n} -> Type)
+  -> refl:(mem -> i:size_nat{i <= v n} -> GTot (a_spec i))
+  -> footprint:(i:size_nat{i <= v n} -> GTot
+      (l:B.loc{B.loc_disjoint l (loc output) /\
+               B.address_liveness_insensitive_locs `B.loc_includes` l}))
+  -> spec:(mem -> GTot (i:size_nat{i < v n} -> a_spec i -> a_spec (i + 1) & Seq.lseq t (v len)))
+  -> impl:(i:size_t{v i < v n} -> Stack unit
+      (requires fun h1 ->
+      	(v i + 1) * v len <= max_size_t /\
+        modifies (footprint (v i) |+| loc (gsub output 0ul (i *! len))) h0 h1)
+//        modifies (B.loc_union (footprint (v i)) (loc output)) h0 h1)
+      (ensures  fun h1 _ h2 ->
+        (let block = gsub output (i *! len) len in
+        let s, b = spec h0 (v i) (refl h1 (v i)) in
+        footprint (v i + 1) `B.loc_includes` footprint (v i) /\
+        B.modifies (B.loc_union (footprint (v i + 1)) (loc block)) h1 h2 /\
+        refl h2 (v i + 1) == s /\ as_seq h2 block == b))) ->
+  Stack unit
+    (requires fun h -> h0 == h /\ live h output)
+    (ensures  fun _ _ h1 ->
+      B.modifies (B.loc_union (footprint (v n)) (loc (gsub output 0ul (n *! len)))) h0 h1 /\
+     (let s, o = Seq.generate_blocks (v len) (v n) a_spec (spec h0) (refl h0 0) in
+      refl h1 (v n) == s /\
+      as_seq #_ #t h1 (gsub output (size 0) (n *! len)) == o))
 
 (** Fill a buffer with a total function *)
 inline_for_extraction
@@ -904,38 +938,42 @@ val mapi:
       modifies1 o h h1 /\
       as_seq h1 o == Seq.mapi (spec_f h0) (as_seq h i))
 
-#set-options "--z3rlimit 50"
-(*
+
+#set-options "--z3rlimit 200"
 inline_for_extraction noextract
 val map_blocks:
     #t:buftype
   -> #a:Type0
-  -> #len:size_t
   -> h0: mem
+  -> len:size_t
   -> blocksize:size_t{v blocksize > 0}
   -> inp:lbuffer_t t a len 
-  -> output:lbuffer a len{eq_or_disjoint inp output}
+  -> output:lbuffer a len
   -> spec_f:(mem -> GTot (i:nat{i < v len / v blocksize} -> Seq.lseq a (v blocksize) -> Seq.lseq a (v blocksize)))
-  -> spec_l:(mem -> GTot (i:nat{i <= v len / v blocksize} -> llen:size_nat{llen < v blocksize} -> Seq.lseq a llen -> Seq.lseq a llen))
+  -> spec_l:(mem -> GTot (i:nat{i == v len / v blocksize} -> llen:size_nat{llen < v blocksize} -> Seq.lseq a llen -> Seq.lseq a llen))
   -> impl_f:(i:size_t{v i < v len / v blocksize} -> Stack unit
-      (requires fun h1 ->	modifies1 (gsub output 0ul (i *. blocksize)) h0 h1)
-      (ensures  fun h1 _ h2 -> 
-	v i * v blocksize + v blocksize <= v len /\
-       (let block = gsub output (i *. blocksize) blocksize in
-	modifies1 block h1 h2 /\
-	as_seq h2 block == spec_f h0 (v i) (as_seq h1 block))))
+      (requires fun h1 -> 
+	(v i + 1) * v blocksize <= max_size_t /\
+        modifies (loc (gsub output 0ul (i *! blocksize))) h0 h1) 
+      (ensures  fun h1 _ h2 ->
+	let iblock = gsub inp (i *! blocksize) blocksize in
+	let oblock = gsub output (i *! blocksize) blocksize in
+        let ob = spec_f h0 (v i) (as_seq h1 iblock) in
+        B.modifies (loc oblock) h1 h2 /\
+        as_seq h2 oblock == ob))
   -> impl_l:(i:size_t{v i == v len / v blocksize} -> Stack unit
-      (requires fun h1 ->	
-	modifies1 (gsub output 0ul (i *. blocksize)) h0 h1)
-      (ensures  fun h1 _ h2 -> 
-	v i * v blocksize + (v len % v blocksize) == v len /\
-       (let block = gsub output (i *. blocksize) (len %. blocksize) in
-	modifies1 block h1 h2 /\
-	as_seq h2 block == spec_l h0 (v i) (v len % v blocksize) (as_seq h1 block))))
+      (requires fun h1 ->
+        modifies (loc (gsub output 0ul (i *! blocksize))) h0 h1)
+      (ensures  fun h1 _ h2 ->
+	let iblock = gsub inp (i *! blocksize) (len %. blocksize)  in
+	let oblock = gsub output (i *! blocksize) (len %. blocksize) in
+        let ob = spec_l h0 (v i) (v len % v blocksize) (as_seq h1 iblock) in
+        B.modifies (loc oblock) h1 h2 /\
+        as_seq h2 oblock == ob)) 
   -> Stack unit
-    (requires fun h -> h0 == h /\ live h output)
+    (requires fun h -> h0 == h /\ live h output /\ live h inp /\ eq_or_disjoint inp output)
     (ensures  fun _ _ h1 -> modifies1 output h0 h1 /\
 	as_seq h1 output == Seq.map_blocks (v blocksize) (as_seq h0 inp) (spec_f h0) (spec_l h0))
 	  
-*)
-  
+
+
